support `#7[.tag]`

src/cddl/spec/ocaml/Parser.ml
@@ -31,6 +31,7 @@ let rbrack = terminal "rbrack" (function RBRACK -> Some () | _ -> None)
 let pound0 = terminal "pound0" (function POUND0 -> Some () | _ -> None)
 let pound1 = terminal "pound1" (function POUND1 -> Some () | _ -> None)
 let pound6 = terminal "pound6" (function POUND6 -> Some () | _ -> None)
+let pound7 = terminal "pound7" (function POUND7 -> Some () | _ -> None)
 let dot = terminal "dot" (function DOT -> Some () | _ -> None)
 let pound = terminal "pound"  (function POUND -> Some () | _ -> None)
 let minus = terminal "minus" (function MINUS -> Some () | _ -> None)
@@ -146,6 +147,7 @@ and type2 () = debug "type2" (
 (* TODO: generalize "#"DIGIT option(tag) *)
       concat pound0 (fun _ -> ret (TElem EUInt));
       concat pound1 (fun _ -> ret (TElem ENInt));
+      concat pound7 (fun _ -> concat (option tag) (fun tag -> ret (match tag with None -> TElem ESimple | Some v -> TElem (ELiteral (LSimple v)))));
       concat pound (fun _ -> ret (TElem EAny));
     ]
 )
